Drafted Classical_Extra (lots of sorry's)

Classical_Extra.thy
@@ -6,212 +6,57 @@ begin
 
 no_notation m_inv ("inv\<index> _" [81] 80)
 
-lemma register_single_valued:
-  assumes registerF: \<open>register F\<close>
-  assumes single: \<open>single_valued a\<close>
-  shows \<open>single_valued (F a)\<close>
-proof -
-  have "mono F"
-    by (simp add: registerF preregister_mono)
-  
-  from single
-  have contains_Id: "a\<inverse> O a \<subseteq> Id"
-    by (auto simp add: single_valued_def)
+lemma register_apply:
+  assumes \<open>register F\<close>
+  shows \<open>Some o register_apply F a = F (Some o a)\<close>
+  sorry
 
-  have "(F a)\<inverse> O F a = F (a\<inverse> O a)"
-    by (metis registerF register_def)
-  also have \<open>\<dots> \<subseteq> F Id\<close>
-    using \<open>mono F\<close> contains_Id
-    by (meson monoD)
-  also have \<open>\<dots> = Id\<close>
-    using registerF register_def by blast
-  
-  finally show "single_valued (F a)"
-    by (auto simp: single_valued_def)
-qed
+lemma register_total:
+  assumes \<open>register F\<close>
+  assumes \<open>dom a = UNIV\<close>
+  shows \<open>dom (F a) = UNIV\<close>
+  sorry
 
+lemma compatible_setter:
+  assumes \<open>register F\<close> and \<open>register G\<close>
+  defines \<open>sF \<equiv> snd (getter_setter F)\<close> and \<open>sG \<equiv> snd (getter_setter G)\<close> 
+  shows \<open>compatible F G \<longleftrightarrow> (\<forall>a b. sF a o sG b = sG b o sF a)\<close>
+  sorry
 
+lemma register_from_getter_setter_compatibleI[intro]:
+  assumes \<open>valid_getter_setter g s\<close>
+  assumes \<open>valid_getter_setter g' s'\<close>
+  assumes \<open>\<And>x y m. s x (s' y m) = s' y (s x m)\<close>
+  shows \<open>compatible (register_from_getter_setter g s) (register_from_getter_setter g' s')\<close>
+  sorry
 
-lemma register_fulldom:
-  assumes registerF: \<open>register F\<close>
-  assumes adom: \<open>Domain a = UNIV\<close>
-  shows \<open>Domain (F a) = UNIV\<close>
-proof -
-  have "mono F"
-    by (simp add: registerF preregister_mono)
-  
-  from adom
-  have contains_Id: "a O a\<inverse> \<supseteq> Id"
-    by (auto simp add: converse_def relcomp_def relcompp_apply)
-  
-  have "F a O (F a)\<inverse> = F (a O a\<inverse>)"
-    by (metis registerF register_def)
-  also have \<open>\<dots> \<supseteq> F Id\<close> (is \<open>_ \<supseteq> \<dots>\<close>)
-    using \<open>mono F\<close> contains_Id
-    by (meson monoD)
-  also have \<open>\<dots> = Id\<close>
-    using registerF register_def by blast
-  
-  finally show "Domain (F a) = UNIV"
-    by auto
-qed
+lemma separating_update1:
+  \<open>separating TYPE(_) {update1 x y | x y. True}\<close>
+  by (smt (verit) mem_Collect_eq separating_def update1_extensionality)
 
+definition "permutation_register (p::'b\<Rightarrow>'a) (a :: 'a update) = map_option (inv p) o a o p"
 
-lemma register_fullrange:
-  assumes registerF: \<open>register F\<close>
-  assumes arange: \<open>Range a = UNIV\<close>
-  shows \<open>Range (F a) = UNIV\<close>
-  using register_fulldom[OF registerF arange[folded Domain_converse]]
-  by (metis Domain_converse registerF register_def)
-
-
-definition "permutation_register (p::'b\<Rightarrow>'a) a = {(inv p x, inv p y)| x y. (x,y) \<in> a}"
-
-lemma permutation_register_hom[simp]: "preregister (permutation_register p)"
+lemma permutation_register_preregister[simp]: "preregister (permutation_register p)"
   unfolding preregister_def
-  apply (rule exI[of _ \<open>{((x,y), (inv p x, inv p y))| x y. True}\<close>])
-  by (auto simp: permutation_register_def[abs_def])
+  sorry
 
 lemma permutation_register_register: 
   fixes p :: "'b \<Rightarrow> 'a"
   assumes "bij p"
   shows "register (permutation_register p)"
-proof (unfold register_def, intro conjI allI)
-  show \<open>preregister (permutation_register p)\<close>
-    by simp
-  show \<open>permutation_register p Id = Id\<close>
-    unfolding permutation_register_def Id_def apply auto
-    by (simp add: assms bij_inv_eq_iff)
-  fix a a'
-  show \<open>permutation_register p a O permutation_register p a' = permutation_register p (a O a')\<close>
-    apply (auto simp: permutation_register_def relcomp_def relcompp_apply)
-    by (metis assms bij_def surj_f_inv_f)
-  show \<open>permutation_register p (a\<inverse>) = (permutation_register p a)\<inverse>\<close>
-    by (auto simp: permutation_register_def)
-qed
+  sorry
 
-definition register_from_setter :: \<open>('b\<Rightarrow>'a) \<Rightarrow> ('a\<Rightarrow>'b\<Rightarrow>'b) \<Rightarrow> ('a,'b) preregister\<close> where
-  \<open>register_from_setter g s a = {(s ax b, s ay b) | b ax ay. (ax,ay) \<in> a}\<close>
-
-lemma register_from_setter_hom[simp]: "preregister (register_from_setter g s)"
-  unfolding preregister_def 
-  apply (rule exI[of _ \<open>{((ax, ay), (s ax b, s ay b))| ax ay b. True}\<close>])
-  apply (rule ext)
-  by (auto simp: register_from_setter_def[abs_def] Image_def[abs_def])
-
-definition "valid_getter_setter g s \<longleftrightarrow> 
-  (\<forall>b. b = s (g b) b) \<and> (\<forall>a b. g (s a b) = a) \<and> (\<forall>a a' b. s a (s a' b) = s a b)"
-
-(* A bit stronger than register_from_setter_register *)
-lemma register_from_setter_register': 
-  fixes s :: "'a \<Rightarrow> 'b \<Rightarrow> 'b" and g :: "'b \<Rightarrow> 'a"
-  assumes \<open>\<And>b. \<exists>b'. b = s (g b) b'\<close>
-  assumes \<open>\<And>a b. g (s a b) = a\<close>
-  assumes \<open>\<And>a a' b1 b2. s a b1 = s a b2 \<Longrightarrow> s a' b1 = s a' b2\<close>
-  shows "register (register_from_setter g s)"
-proof (unfold register_def, intro conjI allI)
-  show \<open>preregister (register_from_setter g s)\<close>
-    by simp
-  show \<open>register_from_setter g s Id = Id\<close>
-    unfolding register_from_setter_def
-    apply (auto simp: register_from_setter_def)
-    using assms by blast
-
-  fix a 
-  show \<open>register_from_setter g s (a\<inverse>) = (register_from_setter g s a)\<inverse>\<close>
-    unfolding register_from_setter_def
-    by (auto simp: register_from_setter_def)
-
-  fix a'
-  show \<open>register_from_setter g s a O register_from_setter g s a' = register_from_setter g s (a O a')\<close>
-    unfolding register_from_setter_def
-    apply (auto simp: register_from_setter_def relcomp_def relcompp_apply)
-    using assms
-    by metis
-qed
-
-
-lemma register_from_setter_register[simp]:
-  fixes s :: "'a \<Rightarrow> 'b \<Rightarrow> 'b" and g :: "'b \<Rightarrow> 'a"
-  assumes "valid_getter_setter g s"
-  shows "register (register_from_setter g s)"
-  apply (rule register_from_setter_register'[where g=g])
-  using assms unfolding valid_getter_setter_def by metis+
-
-lemma register_from_setter_set:
-  assumes "valid_getter_setter g s"
-  shows \<open>register_from_setter g s {(a, a0)|a. True} = {(b, s a0 b)|b. True}\<close>
-  using assms by (auto simp: valid_getter_setter_def register_from_setter_def)
-
-lemma register_from_setter_map:
-  assumes "valid_getter_setter g s"
-  shows \<open>register_from_setter g s {(a, f a)|a. True} = {(b, s (f (g b)) b)|b. True}\<close>
-  using assms by (auto simp: valid_getter_setter_def register_from_setter_def)
-
-
-lemma register_from_setter_compat:
-  assumes [simp]: "valid_getter_setter g1 s1"
-  assumes [simp]: "valid_getter_setter g2 s2"
-  assumes \<open>\<And>a1 a2 b. s1 a1 (s2 a2 b) = s2 a2 (s1 a1 b)\<close>
-  shows \<open>compatible (register_from_setter g1 s1) (register_from_setter g2 s2)\<close>
-  unfolding compatible_def apply simp
-  using assms unfolding valid_getter_setter_def
-  apply (auto simp add: register_from_setter_def relcomp_def relcompp_apply)
-  by metis+
-
-definition setter_from_register :: \<open>('a,'b) preregister \<Rightarrow> ('a \<Rightarrow> 'b \<Rightarrow> 'b)\<close> where
-  \<open>setter_from_register F a' m = (THE m'. (m,m') \<in> F {(a, a') |a. True})\<close>
-
-definition getter_from_register :: \<open>('a,'b) preregister \<Rightarrow> ('b \<Rightarrow> 'a)\<close> where
-  \<open>getter_from_register F m = (THE a. (m,m) \<in> F {(a,a)})\<close>
-
-lemma setter_from_register:
-  assumes \<open>valid_getter_setter g s\<close>
-  shows \<open>setter_from_register (register_from_setter g s) = s\<close>
-  unfolding setter_from_register_def
-  apply (subst register_from_setter_set[OF assms])
-  by auto
-
-lemma getter_from_register:
-  assumes \<open>valid_getter_setter g s\<close>
-  shows \<open>getter_from_register (register_from_setter g s) = g\<close>
-proof -
-  from assms
-  have \<open>\<exists>!a. \<exists>b. m = s a b\<close> for m
-    unfolding valid_getter_setter_def 
-    apply auto by metis
-  with assms show ?thesis
-    unfolding getter_from_register_def register_from_setter_def valid_getter_setter_def 
-    apply (auto intro!:ext)
-    by (smt (verit, ccfv_threshold) Uniq_def the1_equality')
-qed
-
-definition empty_var :: \<open>'a::{CARD_1} rel \<Rightarrow> 'b::finite rel\<close> where
-  "empty_var a = (if a={} then {} else Id)"
+definition empty_var :: \<open>'a::{CARD_1} update \<Rightarrow> 'b update\<close> where
+  "empty_var = register_from_getter_setter (\<lambda>_. undefined) (\<lambda>_ m. m)"
 
 lemma register_empty_var[simp]: \<open>register empty_var\<close>
-proof (unfold register_def, intro conjI allI)
-  show \<open>preregister empty_var\<close>
-    unfolding empty_var_def preregister_def
-    by (rule exI[of _ \<open>UNIV \<times> Id\<close>], rule ext, auto)
-  show \<open>empty_var Id = Id\<close>
-    unfolding empty_var_def by auto
-  fix a b :: "'a update"
-  show \<open>empty_var a O empty_var b = empty_var (a O b)\<close>
-    unfolding empty_var_def apply auto
-    by (metis CARD_1_UNIV Image_singleton_iff empty_iff relcomp.relcompI)
-  show \<open>empty_var (a\<inverse>) = (empty_var a)\<inverse>\<close>
-    unfolding empty_var_def by auto
-qed
+  sorry
 
 lemma empty_var_compatible[simp]: \<open>register X \<Longrightarrow> compatible empty_var X\<close>
-  apply (rule compatibleI)
-  using [[simproc del: compatibility_warn]]
-  by (auto simp: empty_var_def)
+  sorry
 
 lemma empty_var_compatible'[simp]: \<open>register X \<Longrightarrow> compatible X empty_var\<close>
   using compatible_sym empty_var_compatible by blast
-
 
 subsubsection \<open>Example\<close>
 
@@ -219,13 +64,22 @@ record memory =
   x :: "int*int"
   y :: nat
 
-definition "X = register_from_setter x (\<lambda>a b. b\<lparr>x:=a\<rparr>)"
+definition "X = register_from_getter_setter x (\<lambda>a b. b\<lparr>x:=a\<rparr>)"
+definition "Y = register_from_getter_setter y (\<lambda>a b. b\<lparr>y:=a\<rparr>)"
 
-lemma valid: \<open>valid_getter_setter x (\<lambda>a b. b\<lparr>x:=a\<rparr>)\<close>
+lemma validX[simp]: \<open>valid_getter_setter x (\<lambda>a b. b\<lparr>x:=a\<rparr>)\<close>
   unfolding valid_getter_setter_def by auto
 
-lemma register: \<open>register X\<close>
-  by (simp add: valid X_def)
+lemma registerX[simp]: \<open>register X\<close>
+  using X_def register_def validX by blast
 
+lemma validY[simp]: \<open>valid_getter_setter y (\<lambda>a b. b\<lparr>y:=a\<rparr>)\<close>
+  unfolding valid_getter_setter_def by auto
+
+lemma registerY[simp]: \<open>register Y\<close>
+  using Y_def register_def validY by blast
+
+lemma compatibleXY[simp]: \<open>compatible X Y\<close>
+  unfolding X_def Y_def by auto
 
 end
